BananasSafety.thy
@@ -2,402 +2,18 @@ theory BananasSafety
 imports BananasDynamics
 begin
 
-lemma canonical_unit: "\<Gamma> \<turnstile> v : \<one> \<Longrightarrow> v = UnitV"
-  by (cases \<Gamma> v \<one> rule: typecheck\<^sub>v.cases) simp_all
-
-lemma canonical_prod: "\<Gamma> \<turnstile> v : t\<^sub>1 \<otimes> t\<^sub>2 \<Longrightarrow> \<exists>v\<^sub>1 v\<^sub>2. (\<Gamma> \<turnstile> v\<^sub>1 : t\<^sub>1) \<and> (\<Gamma> \<turnstile> v\<^sub>2 : t\<^sub>2) \<and> v = PairV v\<^sub>1 v\<^sub>2"
-  by (cases \<Gamma> v "t\<^sub>1 \<otimes> t\<^sub>2" rule: typecheck\<^sub>v.cases) simp_all
-
-lemma canonical_sum: "\<Gamma> \<turnstile> v : t\<^sub>1 \<oplus> t\<^sub>2 \<Longrightarrow> 
-    \<exists>v'. ((\<Gamma> \<turnstile> v' : t\<^sub>1) \<and> v = InlV v') \<or> ((\<Gamma> \<turnstile> v' : t\<^sub>2) \<and> v = InrV v')"
-  by (cases \<Gamma> v "t\<^sub>1 \<oplus> t\<^sub>2" rule: typecheck\<^sub>v.cases) simp_all
-
-lemma canonical_arrow: "\<Gamma> \<turnstile> v : t\<^sub>1 \<hookrightarrow> t\<^sub>2 \<Longrightarrow> \<exists>e. (\<Gamma> \<turnstile> e : t\<^sub>1 \<rightarrow> t\<^sub>2) \<and> v = FunV e"
-  by (cases \<Gamma> v "t\<^sub>1 \<hookrightarrow> t\<^sub>2" rule: typecheck\<^sub>v.cases) simp_all
-
-lemma canonical_mu: "\<Gamma> \<turnstile> v : \<mu> F \<Longrightarrow> 
-    \<exists>v' n. (\<Gamma> \<turnstile> v' : \<mu> F \<star> F) \<and> v = InjV n v' \<and> var\<^sub>t_type \<Gamma> n = Some F"
-  by (cases \<Gamma> v "\<mu> F" rule: typecheck\<^sub>v.cases) simp_all
-
-theorem progress [simp]: "\<Gamma> \<turnstile> e : t\<^sub>1 \<rightarrow> t\<^sub>2 \<Longrightarrow> \<Gamma> \<turnstile> v : t\<^sub>1 \<Longrightarrow> \<Gamma> \<tturnstile> \<Lambda> \<Longrightarrow> e \<noteq> \<epsilon> \<Longrightarrow> 
-    \<exists>e' v'. \<Lambda> \<turnstile> e \<cdot> v \<leadsto> e' \<cdot> v'"
-    and "\<Gamma> \<turnstile> v : t\<^sub>1 \<Longrightarrow> True"
-  proof (induction \<Gamma> e t\<^sub>1 t\<^sub>2 arbitrary: v rule: typecheck\<^sub>e_typecheck\<^sub>v.inducts)
-  case (tc_con \<Gamma> v\<^sub>2 t\<^sub>2 t\<^sub>1)
-    have "\<Lambda> \<turnstile> \<kappa> v\<^sub>2 \<cdot> v \<leadsto> \<epsilon> \<cdot> v\<^sub>2" by simp
-    thus ?case by fastforce
-  next case (tc_comp \<Gamma> f t\<^sub>2 t\<^sub>3 g)
-    thus ?case
-      proof (cases "g = \<epsilon>")
-      case True
-        hence "\<Lambda> \<turnstile> (f \<cdot> g) \<cdot> v \<leadsto> f \<cdot> v" by simp
-        thus ?thesis by fastforce
-      next case False
-        with tc_comp obtain g' v' where "\<Lambda> \<turnstile> g \<cdot> v \<leadsto> g' \<cdot> v'" by blast
-        with tc_comp have "\<Lambda> \<turnstile> (f \<cdot> g) \<cdot> v \<leadsto> (f \<cdot> g') \<cdot> v'" by simp
-        thus ?thesis by fastforce
-      qed
-  next case tc_fst
-    then obtain v\<^sub>1 v\<^sub>2 where "v = PairV v\<^sub>1 v\<^sub>2" using canonical_prod by blast
-    hence "\<Lambda> \<turnstile> \<pi>\<^sub>1 \<cdot> v \<leadsto> \<epsilon> \<cdot> v\<^sub>1" by simp
-    thus ?case by fastforce
-  next case tc_snd
-    then obtain v\<^sub>1 v\<^sub>2 where "v = PairV v\<^sub>1 v\<^sub>2" using canonical_prod by blast
-    hence "\<Lambda> \<turnstile> \<pi>\<^sub>2 \<cdot> v \<leadsto> \<epsilon> \<cdot> v\<^sub>2" by simp
-    thus ?case by fastforce
-  next case tc_tup
-    hence "\<Lambda> \<turnstile> \<Theta> \<cdot> v \<leadsto> \<epsilon> \<cdot> PairV v v" by simp
-    thus ?case by fastforce
-  next case (tc_pair \<Gamma> f\<^sub>1 t\<^sub>1 t\<^sub>2 f\<^sub>2)
-    then obtain v\<^sub>1 v\<^sub>2 where V: "v = PairV v\<^sub>1 v\<^sub>2" using canonical_prod by blast
-    thus ?case
-      proof (cases "f\<^sub>1 = \<epsilon>")
-      case True note T = True
-        thus ?thesis
-          proof (cases "f\<^sub>2 = \<epsilon>")
-          case True
-            have "\<Lambda> \<turnstile> \<epsilon> \<parallel> \<epsilon> \<cdot> PairV v\<^sub>1 v\<^sub>2 \<leadsto> \<epsilon> \<cdot> PairV v\<^sub>1 v\<^sub>2" by simp
-            with T True V show ?thesis by fastforce
-          next case False
-            with tc_pair V obtain f\<^sub>2' v\<^sub>2' where "\<Lambda> \<turnstile> f\<^sub>2 \<cdot> v\<^sub>2 \<leadsto> f\<^sub>2' \<cdot> v\<^sub>2'" by blast
-            hence "\<Lambda> \<turnstile> \<epsilon> \<parallel> f\<^sub>2 \<cdot> PairV v\<^sub>1 v\<^sub>2 \<leadsto> \<epsilon> \<parallel> f\<^sub>2' \<cdot> PairV v\<^sub>1 v\<^sub>2'" by simp
-            with True V show ?thesis by fastforce
-          qed
-      next case False
-        with tc_pair V obtain f\<^sub>1' v\<^sub>1' where "\<Lambda> \<turnstile> f\<^sub>1 \<cdot> v\<^sub>1 \<leadsto> f\<^sub>1' \<cdot> v\<^sub>1'" by blast    
-        hence "\<Lambda> \<turnstile> f\<^sub>1 \<parallel> f\<^sub>2 \<cdot> PairV v\<^sub>1 v\<^sub>2 \<leadsto> f\<^sub>1' \<parallel> f\<^sub>2 \<cdot> PairV v\<^sub>1' v\<^sub>2" by simp
-        with V show ?thesis by fastforce
-      qed
-  next case tc_inl
-    hence "\<Lambda> \<turnstile> \<iota>\<^sub>l \<cdot> v \<leadsto> \<epsilon> \<cdot> InlV v" by simp
-    thus ?case by fastforce
-  next case tc_inr
-    hence "\<Lambda> \<turnstile> \<iota>\<^sub>r \<cdot> v \<leadsto> \<epsilon> \<cdot> InrV v" by simp
-    thus ?case by fastforce
-  next case tc_str
-    then obtain v' where V: "v = InlV v' \<or> v = InrV v'" using canonical_sum by blast
-    thus ?case
-      proof (cases "v = InlV v'")
-      case True
-        hence "\<Lambda> \<turnstile> \<Xi> \<cdot> v \<leadsto> \<epsilon> \<cdot> v'" by simp
-        thus ?thesis by fastforce
-      next case False
-        with V have "\<Lambda> \<turnstile> \<Xi> \<cdot> v \<leadsto> \<epsilon> \<cdot> v'" by simp
-        thus ?thesis by fastforce
-      qed
-  next case (tc_case \<Gamma> f\<^sub>l t\<^sub>1 t\<^sub>3 f\<^sub>r)
-    then obtain v' where V: "v = InlV v' \<or> v = InrV v'" using canonical_sum by blast
-    thus ?case
-      proof (cases "v = InlV v'")
-      case True
-        hence "\<Lambda> \<turnstile> f\<^sub>l \<bar> f\<^sub>r \<cdot> v \<leadsto> (\<iota>\<^sub>l \<cdot> f\<^sub>l) \<cdot> v'" by simp
-        thus ?thesis by fastforce
-      next case False
-        with V have "\<Lambda> \<turnstile> f\<^sub>l \<bar> f\<^sub>r \<cdot> v \<leadsto> (\<iota>\<^sub>r \<cdot> f\<^sub>r) \<cdot> v'" by simp
-        thus ?thesis by fastforce
-      qed
-  next case tc_dst
-    then obtain v\<^sub>1 v\<^sub>2 where V: "v = PairV (InlV v\<^sub>1) v\<^sub>2 \<or> v = PairV (InrV v\<^sub>1) v\<^sub>2" 
-      using canonical_prod canonical_sum by blast
-    thus ?case
-      proof (cases "v = PairV (InlV v\<^sub>1) v\<^sub>2")
-      case True
-        hence "\<Lambda> \<turnstile> \<rhd> \<cdot> v \<leadsto> \<epsilon> \<cdot> InlV (PairV v\<^sub>1 v\<^sub>2)" by simp
-        thus ?thesis by fastforce
-      next case False
-        with V have "\<Lambda> \<turnstile> \<rhd> \<cdot> v \<leadsto> \<epsilon> \<cdot> InrV (PairV v\<^sub>1 v\<^sub>2)" by simp
-        thus ?thesis by fastforce
-      qed
-  next case tc_app
-    then obtain e v' where V: "v = PairV (FunV e) v'" using canonical_prod canonical_arrow by blast
-    moreover hence "\<Lambda> \<turnstile> $ \<cdot> v \<leadsto> e \<cdot> v'" by simp
-    ultimately show ?case by fastforce
-  next case (tc_arr \<Gamma> f t\<^sub>1 t\<^sub>2 g)
-    then obtain e where "v = FunV e" using canonical_arrow by blast
-    moreover hence "\<Lambda> \<turnstile> g \<leftarrow> f \<cdot> FunV e \<leadsto> \<epsilon> \<cdot> FunV (g \<cdot> e \<cdot> f)" by simp
-    ultimately show ?case by fastforce
-  next case (tc_inj \<Gamma> n)
-    hence "\<Lambda> \<turnstile> \<succ>\<^bsub>n\<^esub> \<cdot> v \<leadsto> \<epsilon> \<cdot> InjV n v" by simp
-    thus ?case by fastforce
-  next case (tc_outj \<Gamma> n F)
-    then obtain v' m where "v = InjV m v' \<and> var\<^sub>t_type \<Gamma> m = Some F" using canonical_mu by blast
-    moreover hence "\<Lambda> \<turnstile> \<prec>\<^bsub>n\<^esub> \<cdot> v \<leadsto> \<epsilon> \<cdot> v'" by simp
-    ultimately show ?case by fastforce
-  next case (tc_cata \<Gamma> n F f t)
-    hence "var\<^sub>t_bind \<Lambda> n = Some F" by (simp add: typecheck_environment_def)
-    hence "\<Lambda> \<turnstile> \<lparr> f \<rparr>\<^bsub>n\<^esub> \<cdot> v \<leadsto> (f \<cdot> \<lparr> f \<rparr>\<^bsub>n\<^esub> \<bullet> F \<cdot> \<prec>\<^bsub>n\<^esub>) \<cdot> v" by simp
-    thus ?case by fastforce
-  next case (tc_ana \<Gamma> n F f t)
-    hence "var\<^sub>t_bind \<Lambda> n = Some F" by (simp add: typecheck_environment_def)
-    hence "\<Lambda> \<turnstile> \<lbrakk> f \<rbrakk>\<^bsub>n\<^esub> \<cdot> v \<leadsto> (\<succ>\<^bsub>n\<^esub> \<cdot> \<lbrakk> f \<rbrakk>\<^bsub>n\<^esub> \<bullet> F \<cdot> f) \<cdot> v" by simp
-    thus ?case by fastforce
-  next case (tc_var \<Gamma> x t\<^sub>1 t\<^sub>2)
-    then obtain e where "var\<^sub>e_bind \<Lambda> x = Some e \<and> \<Gamma> \<turnstile> e : t\<^sub>1 \<rightarrow> t\<^sub>2" 
-      using typecheck_environment_def by fastforce
-    hence "\<Lambda> \<turnstile> Var x \<cdot> v \<leadsto> e \<cdot> v" by simp
-    thus ?case by fastforce
-  qed simp_all
-
-lemma [simp]: "\<Gamma> \<turnstile> e : t\<^sub>1 \<rightarrow> t\<^sub>2 \<Longrightarrow> \<Gamma> \<turnstile> e \<bullet> F : t\<^sub>1 \<star> F \<rightarrow> t\<^sub>2 \<star> F"
-  by (induction e F rule: apply_functor_expr.induct) simp_all
-
-theorem preservation [simp]: "\<Lambda> \<turnstile> e \<cdot> v \<leadsto> e' \<cdot> v' \<Longrightarrow> \<Gamma> \<turnstile> e : t\<^sub>1 \<rightarrow> t\<^sub>2 \<Longrightarrow> 
-    \<Gamma> \<turnstile> v : t\<^sub>1 \<Longrightarrow> \<Gamma> \<tturnstile> \<Lambda> \<Longrightarrow> \<exists>t\<^sub>3. (\<Gamma> \<turnstile> e' : t\<^sub>3 \<rightarrow> t\<^sub>2) \<and> (\<Gamma> \<turnstile> v' : t\<^sub>3)"
-  proof (induction \<Lambda> e v e' v' arbitrary: t\<^sub>1 t\<^sub>2 rule: evaluate.induct)
-  case (ev_con \<Lambda> v\<^sub>1 v\<^sub>2)
-    hence "(\<Gamma> \<turnstile> \<epsilon> : t\<^sub>2 \<rightarrow> t\<^sub>2) \<and> \<Gamma> \<turnstile> v\<^sub>1 : t\<^sub>2" by fastforce
-    thus ?case by fastforce
-  next case (ev_comp1 \<Lambda> g v g' v' f)
-    moreover then obtain t\<^sub>3 where "(\<Gamma> \<turnstile> f : t\<^sub>3 \<rightarrow> t\<^sub>2) \<and> \<Gamma> \<turnstile> g : t\<^sub>1 \<rightarrow> t\<^sub>3" by fastforce
-    ultimately obtain t\<^sub>4 where "(\<Gamma> \<turnstile> f \<cdot> g' : t\<^sub>4 \<rightarrow> t\<^sub>2) \<and> \<Gamma> \<turnstile> v' : t\<^sub>4" by fastforce
-    thus ?case by fastforce
-  next case (ev_fst \<Lambda> v\<^sub>1 v\<^sub>2)
-    hence "(\<Gamma> \<turnstile> \<epsilon> : t\<^sub>2 \<rightarrow> t\<^sub>2) \<and> \<Gamma> \<turnstile> v\<^sub>1 : t\<^sub>2" by fastforce
-    thus ?case by fastforce
-  next case (ev_snd \<Lambda> v\<^sub>1 v\<^sub>2)
-    hence "(\<Gamma> \<turnstile> \<epsilon> : t\<^sub>2 \<rightarrow> t\<^sub>2) \<and> \<Gamma> \<turnstile> v\<^sub>2 : t\<^sub>2" by fastforce
-    thus ?case by fastforce
-  next case (ev_pair1 \<Lambda> f\<^sub>1 v\<^sub>1 f\<^sub>1' v\<^sub>1' f\<^sub>2 v\<^sub>2)
-    then obtain t\<^sub>1\<^sub>1 t\<^sub>1\<^sub>2 t\<^sub>2\<^sub>1 t\<^sub>2\<^sub>2 t\<^sub>1\<^sub>1' where T: "(\<Gamma> \<turnstile> v\<^sub>1 : t\<^sub>1\<^sub>1) \<and> (\<Gamma> \<turnstile> v\<^sub>2 : t\<^sub>1\<^sub>2) \<and> 
-      (\<Gamma> \<turnstile> f\<^sub>1 : t\<^sub>1\<^sub>1 \<rightarrow> t\<^sub>2\<^sub>1) \<and> (\<Gamma> \<turnstile> f\<^sub>2 : t\<^sub>1\<^sub>2 \<rightarrow> t\<^sub>2\<^sub>2) \<and> t\<^sub>1 = t\<^sub>1\<^sub>1 \<otimes> t\<^sub>1\<^sub>2 \<and> t\<^sub>2 = t\<^sub>2\<^sub>1 \<otimes> t\<^sub>2\<^sub>2 \<and> 
-        (\<Gamma> \<turnstile> f\<^sub>1' : t\<^sub>1\<^sub>1' \<rightarrow> t\<^sub>2\<^sub>1) \<and> \<Gamma> \<turnstile> v\<^sub>1' : t\<^sub>1\<^sub>1'" by fastforce
-    hence "(\<Gamma> \<turnstile> f\<^sub>1' \<parallel> f\<^sub>2 : t\<^sub>1\<^sub>1' \<otimes> t\<^sub>1\<^sub>2 \<rightarrow> t\<^sub>2) \<and> \<Gamma> \<turnstile> PairV v\<^sub>1' v\<^sub>2 : t\<^sub>1\<^sub>1' \<otimes> t\<^sub>1\<^sub>2" by simp
-    thus ?case by fastforce
-  next case (ev_pair2 \<Lambda> f\<^sub>2 v\<^sub>2 f\<^sub>2' v\<^sub>2' v\<^sub>1)
-    then obtain t\<^sub>1\<^sub>1 t\<^sub>1\<^sub>2 t\<^sub>2\<^sub>2 t\<^sub>1\<^sub>2' where T: "(\<Gamma> \<turnstile> v\<^sub>1 : t\<^sub>1\<^sub>1) \<and> (\<Gamma> \<turnstile> v\<^sub>2 : t\<^sub>1\<^sub>2) \<and> 
-      (\<Gamma> \<turnstile> f\<^sub>2 : t\<^sub>1\<^sub>2 \<rightarrow> t\<^sub>2\<^sub>2) \<and> t\<^sub>1 = t\<^sub>1\<^sub>1 \<otimes> t\<^sub>1\<^sub>2 \<and> t\<^sub>2 = t\<^sub>1\<^sub>1 \<otimes> t\<^sub>2\<^sub>2 \<and> (\<Gamma> \<turnstile> f\<^sub>2' : t\<^sub>1\<^sub>2' \<rightarrow> t\<^sub>2\<^sub>2) \<and> 
-        \<Gamma> \<turnstile> v\<^sub>2' : t\<^sub>1\<^sub>2'" by fastforce
-    hence "(\<Gamma> \<turnstile> \<epsilon> \<parallel> f\<^sub>2' : t\<^sub>1\<^sub>1 \<otimes> t\<^sub>1\<^sub>2' \<rightarrow> t\<^sub>2) \<and> \<Gamma> \<turnstile> PairV v\<^sub>1 v\<^sub>2' : t\<^sub>1\<^sub>1 \<otimes> t\<^sub>1\<^sub>2'" by simp
-    thus ?case by fastforce
-  next case (ev_pair3 \<Lambda> v\<^sub>1 v\<^sub>2)
-    hence "(\<Gamma> \<turnstile> \<epsilon> : t\<^sub>1 \<rightarrow> t\<^sub>2) \<and> \<Gamma> \<turnstile> PairV v\<^sub>1 v\<^sub>2 : t\<^sub>1" by fastforce
-    thus ?case by fastforce
-  next case (ev_tup \<Lambda> v)
-    hence "t\<^sub>2 = t\<^sub>1 \<otimes> t\<^sub>1" by fastforce
-    moreover from ev_tup have "(\<Gamma> \<turnstile> \<epsilon> : t\<^sub>1 \<otimes> t\<^sub>1 \<rightarrow> t\<^sub>1 \<otimes> t\<^sub>1) \<and> \<Gamma> \<turnstile> PairV v v : t\<^sub>1 \<otimes> t\<^sub>1" 
-      by simp
-    ultimately show ?case by fastforce
-  next case (ev_inl \<Lambda> v)
-    moreover then obtain t\<^sub>3 where "t\<^sub>2 = t\<^sub>1 \<oplus> t\<^sub>3" by fastforce
-    ultimately have "(\<Gamma> \<turnstile> \<epsilon> : t\<^sub>1 \<oplus> t\<^sub>3 \<rightarrow> t\<^sub>2) \<and> \<Gamma> \<turnstile> InlV v : t\<^sub>1 \<oplus> t\<^sub>3" by simp
-    thus ?case by fastforce
-  next case (ev_inr \<Lambda> v)
-    moreover then obtain t\<^sub>3 where "t\<^sub>2 = t\<^sub>3 \<oplus> t\<^sub>1" by fastforce
-    ultimately have "(\<Gamma> \<turnstile> \<epsilon> : t\<^sub>3 \<oplus> t\<^sub>1 \<rightarrow> t\<^sub>2) \<and> \<Gamma> \<turnstile> InrV v : t\<^sub>3 \<oplus> t\<^sub>1" by simp
-    thus ?case by fastforce
-  next case (ev_strl \<Lambda> v)
-    hence "(\<Gamma> \<turnstile> \<epsilon> : t\<^sub>2 \<rightarrow> t\<^sub>2) \<and> \<Gamma> \<turnstile> v : t\<^sub>2" by fastforce
-    thus ?case by fastforce
-  next case (ev_strr \<Lambda> v)
-    hence "(\<Gamma> \<turnstile> \<epsilon> : t\<^sub>2 \<rightarrow> t\<^sub>2) \<and> \<Gamma> \<turnstile> v : t\<^sub>2" by fastforce
-    thus ?case by fastforce
-  next case (ev_csl \<Lambda> f\<^sub>l f\<^sub>r v)
-    then obtain t\<^sub>1\<^sub>l t\<^sub>1\<^sub>r t\<^sub>2\<^sub>l t\<^sub>2\<^sub>r where V: "(\<Gamma> \<turnstile> f\<^sub>l : t\<^sub>1\<^sub>l \<rightarrow> t\<^sub>2\<^sub>l) \<and> (\<Gamma> \<turnstile> f\<^sub>r : t\<^sub>1\<^sub>r \<rightarrow> t\<^sub>2\<^sub>r) \<and> 
-      (\<Gamma> \<turnstile> v : t\<^sub>1\<^sub>l) \<and> t\<^sub>1 = t\<^sub>1\<^sub>l \<oplus> t\<^sub>1\<^sub>r \<and> t\<^sub>2 = t\<^sub>2\<^sub>l \<oplus> t\<^sub>2\<^sub>r" by fastforce
-    hence "\<Gamma> \<turnstile> \<iota>\<^sub>l \<cdot> f\<^sub>l : t\<^sub>1\<^sub>l \<rightarrow> t\<^sub>2\<^sub>l \<oplus> t\<^sub>2\<^sub>r" by (metis tc_inl tc_comp)
-    with V show ?case by fastforce
-  next case (ev_csr \<Lambda> f\<^sub>l f\<^sub>r v)
-    then obtain t\<^sub>1\<^sub>l t\<^sub>1\<^sub>r t\<^sub>2\<^sub>l t\<^sub>2\<^sub>r where V: "(\<Gamma> \<turnstile> f\<^sub>l : t\<^sub>1\<^sub>l \<rightarrow> t\<^sub>2\<^sub>l) \<and> (\<Gamma> \<turnstile> f\<^sub>r : t\<^sub>1\<^sub>r \<rightarrow> t\<^sub>2\<^sub>r) \<and> 
-      (\<Gamma> \<turnstile> v : t\<^sub>1\<^sub>r) \<and> t\<^sub>1 = t\<^sub>1\<^sub>l \<oplus> t\<^sub>1\<^sub>r \<and> t\<^sub>2 = t\<^sub>2\<^sub>l \<oplus> t\<^sub>2\<^sub>r" by fastforce
-    hence "\<Gamma> \<turnstile> \<iota>\<^sub>r \<cdot> f\<^sub>r : t\<^sub>1\<^sub>r \<rightarrow> t\<^sub>2\<^sub>l \<oplus> t\<^sub>2\<^sub>r" by (metis tc_inr tc_comp)
-    with V show ?case by fastforce
-  next case (ev_dstl \<Lambda> v\<^sub>1 v\<^sub>2)
-    then obtain t\<^sub>3 t\<^sub>4 t\<^sub>5 where "(\<Gamma> \<turnstile> v\<^sub>1 : t\<^sub>3) \<and> (\<Gamma> \<turnstile> v\<^sub>2 : t\<^sub>5) \<and> t\<^sub>1 = (t\<^sub>3 \<oplus> t\<^sub>4) \<otimes> t\<^sub>5 \<and> 
-      t\<^sub>2 = t\<^sub>3 \<otimes> t\<^sub>5 \<oplus> t\<^sub>4 \<otimes> t\<^sub>5" by fastforce
-    hence "(\<Gamma> \<turnstile> \<epsilon> : t\<^sub>2 \<rightarrow> t\<^sub>2) \<and> \<Gamma> \<turnstile> InlV (PairV v\<^sub>1 v\<^sub>2) : t\<^sub>2" by simp
-    thus ?case by fastforce
-  next case (ev_dstr \<Lambda> v\<^sub>1 v\<^sub>2)
-    then obtain t\<^sub>3 t\<^sub>4 t\<^sub>5 where "(\<Gamma> \<turnstile> v\<^sub>1 : t\<^sub>4) \<and> (\<Gamma> \<turnstile> v\<^sub>2 : t\<^sub>5) \<and> t\<^sub>1 = (t\<^sub>3 \<oplus> t\<^sub>4) \<otimes> t\<^sub>5 \<and> 
-      t\<^sub>2 = t\<^sub>3 \<otimes> t\<^sub>5 \<oplus> t\<^sub>4 \<otimes> t\<^sub>5" by fastforce
-    hence "(\<Gamma> \<turnstile> \<epsilon> : t\<^sub>2 \<rightarrow> t\<^sub>2) \<and> \<Gamma> \<turnstile> InrV (PairV v\<^sub>1 v\<^sub>2) : t\<^sub>2" by simp
-    thus ?case by fastforce
-  next case (ev_arr \<Lambda> g f e)
-    then obtain t\<^sub>1\<^sub>1 t\<^sub>1\<^sub>2 t\<^sub>2\<^sub>1 t\<^sub>2\<^sub>2 where "(\<Gamma> \<turnstile> f : t\<^sub>2\<^sub>1 \<rightarrow> t\<^sub>1\<^sub>1) \<and> (\<Gamma> \<turnstile> g : t\<^sub>1\<^sub>2 \<rightarrow> t\<^sub>2\<^sub>2) \<and> 
-      (\<Gamma> \<turnstile> e : t\<^sub>1\<^sub>1 \<rightarrow> t\<^sub>1\<^sub>2) \<and> t\<^sub>1 = t\<^sub>1\<^sub>1 \<hookrightarrow> t\<^sub>1\<^sub>2 \<and> t\<^sub>2 = t\<^sub>2\<^sub>1 \<hookrightarrow> t\<^sub>2\<^sub>2" by fastforce
-    hence "(\<Gamma> \<turnstile> \<epsilon> : t\<^sub>2\<^sub>1 \<hookrightarrow> t\<^sub>2\<^sub>2 \<rightarrow> t\<^sub>2) \<and> \<Gamma> \<turnstile> FunV (g \<cdot> e \<cdot> f) : t\<^sub>2\<^sub>1 \<hookrightarrow> t\<^sub>2\<^sub>2" by fastforce
-    thus ?case by fastforce
-  next case (ev_inj \<Lambda> F v)
-    hence "(\<Gamma> \<turnstile> \<epsilon> : t\<^sub>2 \<rightarrow> t\<^sub>2) \<and> \<Gamma> \<turnstile> InjV F v : t\<^sub>2" by fastforce
-    thus ?case by fastforce
-  next case (ev_outj \<Lambda> m F v)
-    hence "(\<Gamma> \<turnstile> \<epsilon> : t\<^sub>2 \<rightarrow> t\<^sub>2) \<and> \<Gamma> \<turnstile> v : t\<^sub>2" by fastforce
-    thus ?case by fastforce
-  next case (ev_cata \<Lambda> n F f v)
-    hence V: "(\<Gamma> \<turnstile> f : t\<^sub>2 \<star> F \<rightarrow> t\<^sub>2) \<and> \<Gamma> \<turnstile> v : \<mu> F" using typecheck_environment_def by fastforce
-    moreover from ev_cata have "\<Gamma> \<turnstile> \<lparr> f \<rparr>\<^bsub>n\<^esub> \<bullet> F : \<mu> F \<star> F \<rightarrow> t\<^sub>2 \<star> F" 
-      using typecheck_environment_def by fastforce
-    moreover from ev_cata have "\<Gamma> \<turnstile> \<prec>\<^bsub>n\<^esub> : \<mu> F \<rightarrow> \<mu> F \<star> F" using typecheck_environment_def by simp
-    ultimately have "\<Gamma> \<turnstile> f \<cdot> \<lparr> f \<rparr>\<^bsub>n\<^esub> \<bullet> F \<cdot> \<prec>\<^bsub>n\<^esub> : \<mu> F \<rightarrow> t\<^sub>2" by (metis tc_comp)
-    with V have "(\<Gamma> \<turnstile> f \<cdot> \<lparr> f \<rparr>\<^bsub>n\<^esub> \<bullet> F \<cdot> \<prec>\<^bsub>n\<^esub> : \<mu> F \<rightarrow> t\<^sub>2) \<and> \<Gamma> \<turnstile> v : \<mu> F" by simp
-    thus ?case by fastforce
-  next case (ev_ana \<Lambda> n F f v)
-    moreover hence V: "(\<Gamma> \<turnstile> f : t\<^sub>1 \<rightarrow> t\<^sub>1 \<star> F) \<and> (\<Gamma> \<turnstile> v : t\<^sub>1) \<and> t\<^sub>2 = \<mu> F"
-      using typecheck_environment_def by fastforce
-    ultimately have "\<Gamma> \<turnstile> \<succ>\<^bsub>n\<^esub> : t\<^sub>2 \<star> F \<rightarrow> t\<^sub>2" using typecheck_environment_def by simp
-    moreover from ev_ana have "\<Gamma> \<turnstile> \<lbrakk> f \<rbrakk>\<^bsub>n\<^esub> \<bullet> F : t\<^sub>1 \<star> F \<rightarrow> t\<^sub>2 \<star> F" by simp
-    moreover from V have "\<Gamma> \<turnstile> f : t\<^sub>1 \<rightarrow> t\<^sub>1 \<star> F" by simp
-    ultimately have "\<Gamma> \<turnstile> \<succ>\<^bsub>n\<^esub> \<cdot> \<lbrakk> f \<rbrakk>\<^bsub>n\<^esub> \<bullet> F \<cdot> f : t\<^sub>1 \<rightarrow> t\<^sub>2" by simp
-    with V show ?case by fastforce
-  next case (ev_var \<Lambda> x e v)
-    hence "var\<^sub>e_type \<Gamma> x = Some (t\<^sub>1, t\<^sub>2)" by fastforce
-    with ev_var obtain e' where "var\<^sub>e_bind \<Lambda> x = Some e' \<and> \<Gamma> \<turnstile> e' : t\<^sub>1 \<rightarrow> t\<^sub>2" 
-      using typecheck_environment_def by fastforce 
-    with ev_var show ?case by fastforce
-  qed fastforce+
-
-(* big-step evaluation *) 
-
-inductive total_eval :: "dynamic_environment \<Rightarrow> expr \<Rightarrow> val \<Rightarrow> val \<Rightarrow> bool" 
-    (infix "\<turnstile> _ \<cdot> _ \<Down>" 60) where
-  tev_base [simp]: "\<Lambda> \<turnstile> \<epsilon> \<cdot> v \<Down> v"
-| tev_step [simp]: "\<Lambda> \<turnstile> e \<cdot> v \<leadsto> e' \<cdot> v' \<Longrightarrow> \<Lambda> \<turnstile> e' \<cdot> v' \<Down> v'' \<Longrightarrow> \<Lambda> \<turnstile> e \<cdot> v \<Down> v''"
-
-lemma [elim]: "\<Lambda> \<turnstile> f \<cdot> v \<Down> v' \<Longrightarrow> \<Lambda> \<turnstile> g \<cdot> v' \<Down> v'' \<Longrightarrow> \<Lambda> \<turnstile> (g \<cdot> f) \<cdot> v \<Down> v''"
-  proof (induction \<Lambda> f v v' rule: total_eval.induct)
-  case (tev_base \<Lambda> v)
-    moreover have "\<Lambda> \<turnstile> (g \<cdot> \<epsilon>) \<cdot> v \<leadsto> g \<cdot> v" by simp
-    ultimately show ?case by (metis tev_step)
-  next case (tev_step \<Lambda> f v f' v' v''')
-    hence "\<Lambda> \<turnstile> (g \<cdot> f) \<cdot> v \<leadsto> (g \<cdot> f') \<cdot> v'" by simp
-    moreover from tev_step have "\<Lambda> \<turnstile> (g \<cdot> f') \<cdot> v' \<Down> v''" by simp
-    ultimately show ?case by (metis total_eval.tev_step)
-  qed
-
-lemma [simp]: "\<Lambda> \<turnstile> e \<cdot> v \<leadsto> \<epsilon> \<cdot> v' \<Longrightarrow> \<Lambda> \<turnstile> e \<cdot> v \<Down> v'"
-  by rule (simp, simp)
-
-lemma eps_big_eval [elim]: "\<Lambda> \<turnstile> \<epsilon> \<cdot> v \<Down> v' \<Longrightarrow> v = v'"
-  proof (induction \<Lambda> \<epsilon> v v' rule: total_eval.induct)
-  case (tev_step \<Lambda> v e' v' v'')
-    thus ?case by (induction \<epsilon> v e' v' rule: evaluate.induct)
-  qed simp_all
-
-lemma [simp]: "\<Lambda> \<turnstile> f\<^sub>2 \<cdot> v\<^sub>2 \<Down> v\<^sub>4 \<Longrightarrow> \<Lambda> \<turnstile> \<epsilon> \<parallel> f\<^sub>2 \<cdot> PairV v\<^sub>1 v\<^sub>2 \<Down> PairV v\<^sub>1 v\<^sub>4"
-  proof (induction \<Lambda> f\<^sub>2 v\<^sub>2 v\<^sub>4 rule: total_eval.induct)
-  case (tev_step \<Lambda> f\<^sub>2 v\<^sub>2 f\<^sub>2' v\<^sub>2' v\<^sub>4)
-    hence "\<Lambda> \<turnstile> \<epsilon> \<parallel> f\<^sub>2 \<cdot> PairV v\<^sub>1 v\<^sub>2 \<leadsto> \<epsilon> \<parallel> f\<^sub>2' \<cdot> PairV v\<^sub>1 v\<^sub>2'" by simp
-    moreover from tev_step have "\<Lambda> \<turnstile> \<epsilon> \<parallel> f\<^sub>2' \<cdot> PairV v\<^sub>1 v\<^sub>2' \<Down> PairV v\<^sub>1 v\<^sub>4" by simp
-    ultimately show ?case by simp
-  qed simp_all
-
-lemma [simp]: "\<Lambda> \<turnstile> f\<^sub>1 \<cdot> v\<^sub>1 \<Down> v\<^sub>3 \<Longrightarrow> \<Lambda> \<turnstile> f\<^sub>2 \<cdot> v\<^sub>2 \<Down> v\<^sub>4 \<Longrightarrow> 
-    \<Lambda> \<turnstile> f\<^sub>1 \<parallel> f\<^sub>2 \<cdot> PairV v\<^sub>1 v\<^sub>2 \<Down> PairV v\<^sub>3 v\<^sub>4"
-  proof (induction \<Lambda> f\<^sub>1 v\<^sub>1 v\<^sub>3 rule: total_eval.induct)
-  case (tev_step \<Lambda> f\<^sub>1 v\<^sub>1 f\<^sub>1' v\<^sub>1' v\<^sub>3)
-    hence "\<Lambda> \<turnstile> f\<^sub>1 \<parallel> f\<^sub>2 \<cdot> PairV v\<^sub>1 v\<^sub>2 \<leadsto> f\<^sub>1' \<parallel> f\<^sub>2 \<cdot> PairV v\<^sub>1' v\<^sub>2" by simp
-    moreover from tev_step have "\<Lambda> \<turnstile> f\<^sub>1' \<parallel> f\<^sub>2 \<cdot> PairV v\<^sub>1' v\<^sub>2 \<Down> PairV v\<^sub>3 v\<^sub>4" by simp
-    ultimately show ?case by simp
-  qed simp_all
-
-lemma pair_big_eval [elim]: "\<Lambda> \<turnstile> f\<^sub>1 \<parallel> f\<^sub>2 \<cdot> PairV v\<^sub>1 v\<^sub>2 \<Down> PairV v\<^sub>3 v\<^sub>4 \<Longrightarrow> 
-    (\<Lambda> \<turnstile> f\<^sub>1 \<cdot> v\<^sub>1 \<Down> v\<^sub>3) \<and> \<Lambda> \<turnstile> f\<^sub>2 \<cdot> v\<^sub>2 \<Down> v\<^sub>4"
-  proof (induction \<Lambda> "f\<^sub>1 \<parallel> f\<^sub>2" "PairV v\<^sub>1 v\<^sub>2" "PairV v\<^sub>3 v\<^sub>4" 
-         arbitrary: f\<^sub>1 f\<^sub>2 v\<^sub>1 v\<^sub>2 rule: total_eval.induct)
-  case (tev_step \<Lambda> e' v')
-    thus ?case
-      proof (induction \<Lambda> "f\<^sub>1 \<parallel> f\<^sub>2" "PairV v\<^sub>1 v\<^sub>2" e' v' arbitrary: f\<^sub>1 f\<^sub>2 v\<^sub>1 v\<^sub>2 rule: evaluate.induct)
-      case (ev_pair3 \<Lambda> v\<^sub>1 v\<^sub>2)
-        hence "PairV v\<^sub>1 v\<^sub>2 = PairV v\<^sub>3 v\<^sub>4" by (metis eps_big_eval)
-        thus ?case by simp
-      qed simp_all
-  qed
-
-lemma [simp]: "\<Lambda> \<turnstile> f\<^sub>l \<cdot> v \<Down> v' \<Longrightarrow> \<Lambda> \<turnstile> f\<^sub>l \<bar> f\<^sub>r \<cdot> InlV v \<Down> InlV v'"
-  proof
-    show "\<Lambda> \<turnstile> f\<^sub>l \<bar> f\<^sub>r \<cdot> InlV v \<leadsto> (\<iota>\<^sub>l \<cdot> f\<^sub>l) \<cdot> v" by simp
-    show "\<Lambda> \<turnstile> f\<^sub>l \<cdot> v \<Down> v' \<Longrightarrow> \<Lambda> \<turnstile> (\<iota>\<^sub>l \<cdot> f\<^sub>l) \<cdot> v \<Down> InlV v'" by auto
-  qed
-
-lemma [simp]: "\<Lambda> \<turnstile> f\<^sub>r \<cdot> v \<Down> v' \<Longrightarrow> \<Lambda> \<turnstile> f\<^sub>l \<bar> f\<^sub>r \<cdot> InrV v \<Down> InrV v'"
-  proof
-    show "\<Lambda> \<turnstile> f\<^sub>l \<bar> f\<^sub>r \<cdot> InrV v \<leadsto> (\<iota>\<^sub>r \<cdot> f\<^sub>r) \<cdot> v" by simp
-    show "\<Lambda> \<turnstile> f\<^sub>r \<cdot> v \<Down> v' \<Longrightarrow> \<Lambda> \<turnstile> (\<iota>\<^sub>r \<cdot> f\<^sub>r) \<cdot> v \<Down> InrV v'" by auto
-  qed
-
-(* since we are a turing-complete language, total progress is not provable *)
-
-theorem total_preservation [simp]: "\<Lambda> \<turnstile> e \<cdot> v \<Down> v' \<Longrightarrow> \<Gamma> \<turnstile> e : t\<^sub>1 \<rightarrow> t\<^sub>2 \<Longrightarrow> 
-    \<Gamma> \<turnstile> v : t\<^sub>1 \<Longrightarrow> \<Gamma> \<tturnstile> \<Lambda> \<Longrightarrow> \<Gamma> \<turnstile> v' : t\<^sub>2"
-  proof (induction \<Lambda> e v v' arbitrary: t\<^sub>1 rule: total_eval.induct)
-  case (tev_step \<Lambda> e v e' v' v'')
-    moreover then obtain t\<^sub>3 where "(\<Gamma> \<turnstile> e' : t\<^sub>3 \<rightarrow> t\<^sub>2) \<and> (\<Gamma> \<turnstile> v' : t\<^sub>3)" 
-      by (metis preservation)
-    ultimately show ?case by fastforce
-  qed auto
-
 (* environment lemmas *)
 
+lemma [simp]: "combine\<^sub>d empty_dynamic \<Lambda> = \<Lambda>"
+  by (simp add: combine\<^sub>d_def empty_dynamic_def)
 
+lemma [simp]: "combine\<^sub>d \<Lambda> empty_dynamic = \<Lambda>"
+  by (simp add: combine\<^sub>d_def empty_dynamic_def)
 
-lemma [simp]: "\<Gamma> \<turnstile> e : t\<^sub>1 \<rightarrow> t\<^sub>2 \<Longrightarrow> x \<notin> dom (var\<^sub>e_type \<Gamma>) \<Longrightarrow> 
-    \<Gamma>\<lparr>var\<^sub>e_type := var\<^sub>e_type \<Gamma>(x \<mapsto> (tt\<^sub>1, tt\<^sub>2))\<rparr> \<turnstile> e : t\<^sub>1 \<rightarrow> t\<^sub>2"
-  and [simp]: "\<Gamma> \<turnstile> v : t \<Longrightarrow> x \<notin> dom (var\<^sub>e_type \<Gamma>) \<Longrightarrow> 
-    \<Gamma>\<lparr>var\<^sub>e_type := var\<^sub>e_type \<Gamma>(x \<mapsto> (tt\<^sub>1, tt\<^sub>2))\<rparr> \<turnstile> v : t"
-  proof (induction \<Gamma> e t\<^sub>1 t\<^sub>2 and \<Gamma> v t rule: typecheck\<^sub>e_typecheck\<^sub>v.inducts) 
-  case (tc_var \<Gamma> y t\<^sub>1 t\<^sub>2)
-    hence "(var\<^sub>e_type \<Gamma>(x \<mapsto> (tt\<^sub>1, tt\<^sub>2))) y = Some (t\<^sub>1, t\<^sub>2)" by auto
-    hence "\<Gamma>\<lparr>var\<^sub>e_type := var\<^sub>e_type \<Gamma>(x \<mapsto> (tt\<^sub>1, tt\<^sub>2))\<rparr> \<turnstile> Var y : t\<^sub>1 \<rightarrow> t\<^sub>2" by simp
-    thus ?case by blast
-  qed simp_all
-
-lemma [simp]: "\<Gamma> \<turnstile> e : t\<^sub>1 \<rightarrow> t\<^sub>2 \<Longrightarrow> x \<notin> dom (var\<^sub>v_type \<Gamma>) \<Longrightarrow> 
-    \<Gamma>\<lparr>var\<^sub>v_type := var\<^sub>v_type \<Gamma>(x \<mapsto> tt)\<rparr> \<turnstile> e : t\<^sub>1 \<rightarrow> t\<^sub>2"
-  and [simp]: "\<Gamma> \<turnstile> v : t \<Longrightarrow> x \<notin> dom (var\<^sub>v_type \<Gamma>) \<Longrightarrow> \<Gamma>\<lparr>var\<^sub>v_type := var\<^sub>v_type \<Gamma>(x \<mapsto> tt)\<rparr> \<turnstile> v : t"
-  by (induction \<Gamma> e t\<^sub>1 t\<^sub>2 and \<Gamma> v t rule: typecheck\<^sub>e_typecheck\<^sub>v.inducts) simp_all
+lemma [simp]: "combine\<^sub>d (combine\<^sub>d \<Lambda>\<^sub>1 \<Lambda>\<^sub>2) \<Lambda>\<^sub>3 = combine\<^sub>d \<Lambda>\<^sub>1 (combine\<^sub>d \<Lambda>\<^sub>2 \<Lambda>\<^sub>3)"
+  by (simp add: combine\<^sub>d_def empty_dynamic_def)
 
 (*
-
-lemma [simp]: "\<Gamma> \<turnstile> e : t\<^sub>1 \<rightarrow> t\<^sub>2 \<Longrightarrow> domain\<^sub>s \<Gamma> \<inter> domain\<^sub>s \<Gamma>' = {} \<Longrightarrow> combine\<^sub>s \<Gamma> \<Gamma>' \<turnstile> e : t\<^sub>1 \<rightarrow> t\<^sub>2"
-  and [simp]: "\<Gamma> \<turnstile> v : t \<Longrightarrow> domain\<^sub>s \<Gamma> \<inter> domain\<^sub>s \<Gamma>' = {} \<Longrightarrow> combine\<^sub>s \<Gamma> \<Gamma>' \<turnstile> v : t"
-  by (induction \<Gamma> e t\<^sub>1 t\<^sub>2 and \<Gamma> v t rule: typecheck\<^sub>e_typecheck\<^sub>v.inducts) simp_all
-
-lemma [simp]: "\<And>xa t\<^sub>1' t\<^sub>2'.
-       \<Gamma> \<turnstile> e : t\<^sub>1 \<rightarrow> t\<^sub>2 \<Longrightarrow>
-       var\<^sub>t_type \<Gamma> = var\<^sub>t_bind \<Lambda> \<Longrightarrow>
-       dom (var\<^sub>e_type \<Gamma>) = dom (var\<^sub>e_bind \<Lambda>) \<Longrightarrow>
-       var\<^sub>e_bind \<Lambda> x = None \<Longrightarrow>
-       var\<^sub>v_type \<Gamma> x = None \<Longrightarrow>
-       \<forall>x t\<^sub>1 t\<^sub>2. var\<^sub>e_type \<Gamma> x = Some (t\<^sub>1, t\<^sub>2) \<longrightarrow> (\<exists>e. var\<^sub>e_bind \<Lambda> x = Some e \<and> \<Gamma> \<turnstile> e : t\<^sub>1 \<rightarrow> t\<^sub>2) \<Longrightarrow>
-       \<forall>x t. var\<^sub>v_type \<Gamma> x = Some t \<longrightarrow> (\<exists>v. var\<^sub>v_bind \<Lambda> x = Some v \<and> \<Gamma> \<turnstile> v : t) \<Longrightarrow>
-       var\<^sub>t_bind \<Lambda> x = None \<Longrightarrow>
-       xa \<noteq> x \<Longrightarrow>
-       var\<^sub>e_type \<Gamma> xa = Some (t\<^sub>1', t\<^sub>2') \<Longrightarrow>
-       \<exists>e. var\<^sub>e_bind \<Lambda> xa = Some e \<and> \<Gamma>\<lparr>var\<^sub>e_type := var\<^sub>e_type \<Gamma>(x \<mapsto> (t\<^sub>1, t\<^sub>2))\<rparr> \<turnstile> e : t\<^sub>1' \<rightarrow> t\<^sub>2'"
-  by simp
-
-lemma [simp]: "\<And>xa t. \<Gamma> \<turnstile> e : t\<^sub>1 \<rightarrow> t\<^sub>2 \<Longrightarrow>
-            var\<^sub>t_type \<Gamma> = var\<^sub>t_bind \<Lambda> \<Longrightarrow>
-            dom (var\<^sub>e_type \<Gamma>) = dom (var\<^sub>e_bind \<Lambda>) \<Longrightarrow>
-            var\<^sub>e_bind \<Lambda> x = None \<Longrightarrow>
-            var\<^sub>v_type \<Gamma> x = None \<Longrightarrow>
-            \<forall>x t\<^sub>1 t\<^sub>2. var\<^sub>e_type \<Gamma> x = Some (t\<^sub>1, t\<^sub>2) \<longrightarrow> (\<exists>e. var\<^sub>e_bind \<Lambda> x = Some e \<and> \<Gamma> \<turnstile> e : t\<^sub>1 \<rightarrow> t\<^sub>2) \<Longrightarrow>
-            \<forall>x t. var\<^sub>v_type \<Gamma> x = Some t \<longrightarrow> (\<exists>v. var\<^sub>v_bind \<Lambda> x = Some v \<and> \<Gamma> \<turnstile> v : t) \<Longrightarrow>
-            var\<^sub>t_bind \<Lambda> x = None \<Longrightarrow>
-            var\<^sub>v_type \<Gamma> xa = Some t \<Longrightarrow> \<exists>v. var\<^sub>v_bind \<Lambda> xa = Some v \<and> \<Gamma>\<lparr>var\<^sub>e_type := var\<^sub>e_type \<Gamma>(x \<mapsto> (t\<^sub>1, t\<^sub>2))\<rparr> \<turnstile> v : t"
-  by simp
-
-lemma [simp]: "\<And>xa t\<^sub>1 t\<^sub>2.
-       \<Gamma> \<turnstile> v : t \<Longrightarrow>
-       var\<^sub>t_type \<Gamma> = var\<^sub>t_bind \<Lambda> \<Longrightarrow>
-       dom (var\<^sub>e_type \<Gamma>) = dom (var\<^sub>e_bind \<Lambda>) \<Longrightarrow>
-       var\<^sub>e_bind \<Lambda> x = None \<Longrightarrow>
-       var\<^sub>v_type \<Gamma> x = None \<Longrightarrow>
-       \<forall>x t\<^sub>1 t\<^sub>2. var\<^sub>e_type \<Gamma> x = Some (t\<^sub>1, t\<^sub>2) \<longrightarrow> (\<exists>e. var\<^sub>e_bind \<Lambda> x = Some e \<and> \<Gamma> \<turnstile> e : t\<^sub>1 \<rightarrow> t\<^sub>2) \<Longrightarrow>
-       \<forall>x t. var\<^sub>v_type \<Gamma> x = Some t \<longrightarrow> (\<exists>v. var\<^sub>v_bind \<Lambda> x = Some v \<and> \<Gamma> \<turnstile> v : t) \<Longrightarrow>
-       var\<^sub>t_bind \<Lambda> x = None \<Longrightarrow>
-       var\<^sub>e_type \<Gamma> xa = Some (t\<^sub>1, t\<^sub>2) \<Longrightarrow> \<exists>e. var\<^sub>e_bind \<Lambda> xa = Some e \<and> \<Gamma>\<lparr>var\<^sub>v_type := var\<^sub>v_type \<Gamma>(x \<mapsto> t)\<rparr> \<turnstile> e : t\<^sub>1 \<rightarrow> t\<^sub>2"
-  by simp
-
-lemma [simp]: "\<And>xa ta. \<Gamma> \<turnstile> v : t \<Longrightarrow>
-             var\<^sub>t_type \<Gamma> = var\<^sub>t_bind \<Lambda> \<Longrightarrow>
-             dom (var\<^sub>e_type \<Gamma>) = dom (var\<^sub>e_bind \<Lambda>) \<Longrightarrow>
-             var\<^sub>e_bind \<Lambda> x = None \<Longrightarrow>
-             var\<^sub>v_type \<Gamma> x = None \<Longrightarrow>
-             \<forall>x t\<^sub>1 t\<^sub>2. var\<^sub>e_type \<Gamma> x = Some (t\<^sub>1, t\<^sub>2) \<longrightarrow> (\<exists>e. var\<^sub>e_bind \<Lambda> x = Some e \<and> \<Gamma> \<turnstile> e : t\<^sub>1 \<rightarrow> t\<^sub>2) \<Longrightarrow>
-             \<forall>x t. var\<^sub>v_type \<Gamma> x = Some t \<longrightarrow> (\<exists>v. var\<^sub>v_bind \<Lambda> x = Some v \<and> \<Gamma> \<turnstile> v : t) \<Longrightarrow>
-             var\<^sub>t_bind \<Lambda> x = None \<Longrightarrow>
-             xa \<noteq> x \<Longrightarrow> var\<^sub>v_type \<Gamma> xa = Some ta \<Longrightarrow> \<exists>v. var\<^sub>v_bind \<Lambda> xa = Some v \<and> \<Gamma>\<lparr>var\<^sub>v_type := var\<^sub>v_type \<Gamma>(x \<mapsto> t)\<rparr> \<turnstile> v : ta"
-  by simp *)
 
 lemma [simp]: "\<Gamma> \<turnstile> e : t\<^sub>1 \<rightarrow> t\<^sub>2 \<Longrightarrow> \<Gamma> \<tturnstile> \<Lambda> \<Longrightarrow> x \<notin> domain\<^sub>s \<Gamma> \<Longrightarrow> 
     extend\<^sub>e\<^sub>s x (t\<^sub>1, t\<^sub>2) \<Gamma> \<tturnstile> extend\<^sub>e\<^sub>d x e \<Lambda>"
@@ -410,22 +26,13 @@ lemma typecheck_combine [simp]: "\<Gamma> \<tturnstile> \<Lambda> \<Longrightarr
     combine\<^sub>s \<Gamma> \<Gamma>' \<tturnstile> combine\<^sub>d \<Lambda> \<Lambda>'"
   by (auto simp add: typecheck_environment_def combine\<^sub>s_def combine\<^sub>d_def domain\<^sub>s_def)
 
-lemma [simp]: "combine\<^sub>d empty_dynamic \<Lambda> = \<Lambda>"
-  by (simp add: combine\<^sub>d_def empty_dynamic_def)
-
-lemma [simp]: "combine\<^sub>d \<Lambda> empty_dynamic = \<Lambda>"
-  by (simp add: combine\<^sub>d_def empty_dynamic_def)
-
-lemma [simp]: "combine\<^sub>d (combine\<^sub>d \<Lambda>\<^sub>1 \<Lambda>\<^sub>2) \<Lambda>\<^sub>3 = combine\<^sub>d \<Lambda>\<^sub>1 (combine\<^sub>d \<Lambda>\<^sub>2 \<Lambda>\<^sub>3)"
-  by (simp add: combine\<^sub>d_def empty_dynamic_def)
-
 lemma [simp]: "combine\<^sub>d \<Lambda> (empty_dynamic\<lparr>var\<^sub>e_bind := [x \<mapsto> e]\<rparr>) = extend\<^sub>e\<^sub>d x e \<Lambda>"
   by (simp add: combine\<^sub>d_def empty_dynamic_def extend\<^sub>e\<^sub>d_def)
 
 lemma [simp]: "combine\<^sub>d \<Lambda> (empty_dynamic\<lparr>var\<^sub>v_bind := [x \<mapsto> v]\<rparr>) = extend\<^sub>v\<^sub>d x v \<Lambda>"
   by (simp add: combine\<^sub>d_def empty_dynamic_def extend\<^sub>v\<^sub>d_def)
 
-lemma [simp]: "typecheck\<^sub>c\<^sub>e \<Gamma> F cts x = Some (t\<^sub>1, t\<^sub>2) \<Longrightarrow> \<exists>e. assemble_context\<^sub>c\<^sub>e n d cts x = Some e"
+lemma [simp]: "typecheck\<^sub>c\<^sub>e \<Gamma> F cts x = Some (t\<^sub>1, t\<^sub>2) \<Longrightarrow> \<exists>e. assemble_context\<^sub>c\<^sub>e \<Gamma> n d cts x = Some e"
   by (induction F cts x arbitrary: d rule: typecheck\<^sub>c\<^sub>e.induct) auto
 
 lemma [simp]: "assemble_context\<^sub>c\<^sub>e n d cts x = Some e \<Longrightarrow> \<exists>t\<^sub>1 t\<^sub>2. typecheck\<^sub>c\<^sub>e \<Gamma> F cts x = Some (t\<^sub>1, t\<^sub>2)"
@@ -547,17 +154,16 @@ lemma [simp]: "\<Gamma>\<^sub>1 \<Turnstile> \<delta> : \<Gamma>\<^sub>2 \<Longr
   case (tcd_type \<Gamma> x cts)
     hence "domain\<^sub>s \<Gamma> \<inter> domain\<^sub>s (typecheck\<^sub>d x cts) = {}" by auto
     with tcd_type show ?case by (metis typecheck_combine tc_typedecl)
-  qed simp_all
+  qed simp_all *)
 
 lemma tc_defs_parts [simp]: "\<Gamma>\<^sub>1 \<Turnstile> \<Lambda>\<^sub>2 :: \<Gamma>\<^sub>2 \<Longrightarrow> \<Gamma>\<^sub>1 \<tturnstile> \<Lambda>\<^sub>1 \<Longrightarrow> \<Gamma>\<^sub>2 \<tturnstile> combine\<^sub>d \<Lambda>\<^sub>1 (assemble_context \<Lambda>\<^sub>2)"
   proof (induction \<Gamma>\<^sub>1 \<Lambda>\<^sub>2 \<Gamma>\<^sub>2 arbitrary: \<Lambda>\<^sub>1 rule: typecheck_decls.induct)
   case (tcd_cons \<Gamma>\<^sub>1 \<delta> \<Gamma>\<^sub>2 \<Lambda>\<^sub>2 \<Gamma>\<^sub>3)
-    moreover hence "\<Gamma>\<^sub>2 \<tturnstile> combine\<^sub>d \<Lambda>\<^sub>1 (assemble_context' \<delta>)" by simp
-    ultimately show ?case by fastforce
+    thus ?case by simp
   qed simp_all
 
 lemma [simp]: "empty_static \<tturnstile> empty_dynamic" 
-  by (simp add: typecheck_environment_def empty_static_def empty_dynamic_def)
+  by (simp add: typecheck_environment_def empty_static_def empty_dynamic_def typecheck_env\<^sub>e_def typecheck_env\<^sub>v_def)
 
 lemma [simp]: "empty_static \<Turnstile> \<Lambda> :: \<Gamma> \<Longrightarrow> \<Gamma> \<tturnstile> assemble_context \<Lambda>"
   proof -
@@ -565,7 +171,145 @@ lemma [simp]: "empty_static \<Turnstile> \<Lambda> :: \<Gamma> \<Longrightarrow>
     moreover have "empty_static \<tturnstile> empty_dynamic" by simp
     ultimately have "\<Gamma> \<tturnstile> combine\<^sub>d empty_dynamic (assemble_context \<Lambda>)" by (metis tc_defs_parts)
     thus "\<Gamma> \<tturnstile> assemble_context \<Lambda>" by simp
-  qed                                                                  
+  qed
+
+(* progress *)
+
+lemma canonical_unit: "\<Gamma> \<turnstile> v : \<one> \<Longrightarrow> v = UnitV"
+  by (cases \<Gamma> v \<one> rule: typecheck\<^sub>v.cases) simp_all
+
+lemma canonical_prod: "\<Gamma> \<turnstile> v : t\<^sub>1 \<otimes> t\<^sub>2 \<Longrightarrow> \<exists>v\<^sub>1 v\<^sub>2. (\<Gamma> \<turnstile> v\<^sub>1 : t\<^sub>1) \<and> (\<Gamma> \<turnstile> v\<^sub>2 : t\<^sub>2) \<and> v = PairV v\<^sub>1 v\<^sub>2"
+  by (cases \<Gamma> v "t\<^sub>1 \<otimes> t\<^sub>2" rule: typecheck\<^sub>v.cases) simp_all
+
+lemma canonical_sum: "\<Gamma> \<turnstile> v : t\<^sub>1 \<oplus> t\<^sub>2 \<Longrightarrow> 
+    \<exists>v'. ((\<Gamma> \<turnstile> v' : t\<^sub>1) \<and> v = InlV v') \<or> ((\<Gamma> \<turnstile> v' : t\<^sub>2) \<and> v = InrV v')"
+  by (cases \<Gamma> v "t\<^sub>1 \<oplus> t\<^sub>2" rule: typecheck\<^sub>v.cases) simp_all
+
+lemma canonical_arrow: "\<Gamma> \<turnstile> v : t\<^sub>1 \<hookrightarrow> t\<^sub>2 \<Longrightarrow> \<exists>e. (\<Gamma> \<turnstile> e : t\<^sub>1 \<rightarrow> t\<^sub>2) \<and> v = FunV e"
+  by (cases \<Gamma> v "t\<^sub>1 \<hookrightarrow> t\<^sub>2" rule: typecheck\<^sub>v.cases) simp_all
+
+lemma canonical_mu: "\<Gamma> \<turnstile> v : \<mu> F \<Longrightarrow> 
+    \<exists>v' n. (\<Gamma> \<turnstile> v' : \<mu> F \<star> F) \<and> v = InjV n v' \<and> var\<^sub>t_type \<Gamma> n = Some F"
+  by (cases \<Gamma> v "\<mu> F" rule: typecheck\<^sub>v.cases) simp_all
+
+theorem expr_progress [simp]: "\<Gamma> \<turnstile> e : t\<^sub>1 \<rightarrow> t\<^sub>2 \<Longrightarrow> \<Gamma> \<turnstile> v : t\<^sub>1 \<Longrightarrow> \<Gamma> \<tturnstile> \<Lambda> \<Longrightarrow> e \<noteq> \<epsilon> \<Longrightarrow> 
+    \<exists>e' v'. \<Lambda> \<turnstile> e \<cdot> v \<leadsto> e' \<cdot> v'"
+    and "\<Gamma> \<turnstile> v : t\<^sub>1 \<Longrightarrow> True"
+  proof (induction \<Gamma> e t\<^sub>1 t\<^sub>2 arbitrary: v rule: typecheck\<^sub>e_typecheck\<^sub>v.inducts)
+  case (tc_con \<Gamma> v\<^sub>2 t\<^sub>2 t\<^sub>1)
+    have "\<Lambda> \<turnstile> \<kappa> v\<^sub>2 \<cdot> v \<leadsto> \<epsilon> \<cdot> v\<^sub>2" by simp
+    thus ?case by fastforce
+  next case (tc_comp \<Gamma> f t\<^sub>2 t\<^sub>3 g)
+    thus ?case
+      proof (cases "g = \<epsilon>")
+      case True
+        hence "\<Lambda> \<turnstile> (f \<cdot> g) \<cdot> v \<leadsto> f \<cdot> v" by simp
+        thus ?thesis by fastforce
+      next case False
+        with tc_comp obtain g' v' where "\<Lambda> \<turnstile> g \<cdot> v \<leadsto> g' \<cdot> v'" by blast
+        with tc_comp have "\<Lambda> \<turnstile> (f \<cdot> g) \<cdot> v \<leadsto> (f \<cdot> g') \<cdot> v'" by simp
+        thus ?thesis by fastforce
+      qed
+  next case tc_fst
+    then obtain v\<^sub>1 v\<^sub>2 where "v = PairV v\<^sub>1 v\<^sub>2" using canonical_prod by blast
+    hence "\<Lambda> \<turnstile> \<pi>\<^sub>1 \<cdot> v \<leadsto> \<epsilon> \<cdot> v\<^sub>1" by simp
+    thus ?case by fastforce
+  next case tc_snd
+    then obtain v\<^sub>1 v\<^sub>2 where "v = PairV v\<^sub>1 v\<^sub>2" using canonical_prod by blast
+    hence "\<Lambda> \<turnstile> \<pi>\<^sub>2 \<cdot> v \<leadsto> \<epsilon> \<cdot> v\<^sub>2" by simp
+    thus ?case by fastforce
+  next case tc_tup
+    hence "\<Lambda> \<turnstile> \<Theta> \<cdot> v \<leadsto> \<epsilon> \<cdot> PairV v v" by simp
+    thus ?case by fastforce
+  next case (tc_pair \<Gamma> f\<^sub>1 t\<^sub>1 t\<^sub>2 f\<^sub>2)
+    then obtain v\<^sub>1 v\<^sub>2 where V: "v = PairV v\<^sub>1 v\<^sub>2" using canonical_prod by blast
+    thus ?case
+      proof (cases "f\<^sub>1 = \<epsilon>")
+      case True note T = True
+        thus ?thesis
+          proof (cases "f\<^sub>2 = \<epsilon>")
+          case True
+            have "\<Lambda> \<turnstile> \<epsilon> \<parallel> \<epsilon> \<cdot> PairV v\<^sub>1 v\<^sub>2 \<leadsto> \<epsilon> \<cdot> PairV v\<^sub>1 v\<^sub>2" by simp
+            with T True V show ?thesis by fastforce
+          next case False
+            with tc_pair V obtain f\<^sub>2' v\<^sub>2' where "\<Lambda> \<turnstile> f\<^sub>2 \<cdot> v\<^sub>2 \<leadsto> f\<^sub>2' \<cdot> v\<^sub>2'" by blast
+            hence "\<Lambda> \<turnstile> \<epsilon> \<parallel> f\<^sub>2 \<cdot> PairV v\<^sub>1 v\<^sub>2 \<leadsto> \<epsilon> \<parallel> f\<^sub>2' \<cdot> PairV v\<^sub>1 v\<^sub>2'" by simp
+            with True V show ?thesis by fastforce
+          qed
+      next case False
+        with tc_pair V obtain f\<^sub>1' v\<^sub>1' where "\<Lambda> \<turnstile> f\<^sub>1 \<cdot> v\<^sub>1 \<leadsto> f\<^sub>1' \<cdot> v\<^sub>1'" by blast    
+        hence "\<Lambda> \<turnstile> f\<^sub>1 \<parallel> f\<^sub>2 \<cdot> PairV v\<^sub>1 v\<^sub>2 \<leadsto> f\<^sub>1' \<parallel> f\<^sub>2 \<cdot> PairV v\<^sub>1' v\<^sub>2" by simp
+        with V show ?thesis by fastforce
+      qed
+  next case tc_inl
+    hence "\<Lambda> \<turnstile> \<iota>\<^sub>l \<cdot> v \<leadsto> \<epsilon> \<cdot> InlV v" by simp
+    thus ?case by fastforce
+  next case tc_inr
+    hence "\<Lambda> \<turnstile> \<iota>\<^sub>r \<cdot> v \<leadsto> \<epsilon> \<cdot> InrV v" by simp
+    thus ?case by fastforce
+  next case tc_str
+    then obtain v' where V: "v = InlV v' \<or> v = InrV v'" using canonical_sum by blast
+    thus ?case
+      proof (cases "v = InlV v'")
+      case True
+        hence "\<Lambda> \<turnstile> \<Xi> \<cdot> v \<leadsto> \<epsilon> \<cdot> v'" by simp
+        thus ?thesis by fastforce
+      next case False
+        with V have "\<Lambda> \<turnstile> \<Xi> \<cdot> v \<leadsto> \<epsilon> \<cdot> v'" by simp
+        thus ?thesis by fastforce
+      qed
+  next case (tc_case \<Gamma> f\<^sub>l t\<^sub>1 t\<^sub>3 f\<^sub>r)
+    then obtain v' where V: "v = InlV v' \<or> v = InrV v'" using canonical_sum by blast
+    thus ?case
+      proof (cases "v = InlV v'")
+      case True
+        hence "\<Lambda> \<turnstile> f\<^sub>l \<bar> f\<^sub>r \<cdot> v \<leadsto> (\<iota>\<^sub>l \<cdot> f\<^sub>l) \<cdot> v'" by simp
+        thus ?thesis by fastforce
+      next case False
+        with V have "\<Lambda> \<turnstile> f\<^sub>l \<bar> f\<^sub>r \<cdot> v \<leadsto> (\<iota>\<^sub>r \<cdot> f\<^sub>r) \<cdot> v'" by simp
+        thus ?thesis by fastforce
+      qed
+  next case tc_dst
+    then obtain v\<^sub>1 v\<^sub>2 where V: "v = PairV (InlV v\<^sub>1) v\<^sub>2 \<or> v = PairV (InrV v\<^sub>1) v\<^sub>2" 
+      using canonical_prod canonical_sum by blast
+    thus ?case
+      proof (cases "v = PairV (InlV v\<^sub>1) v\<^sub>2")
+      case True
+        hence "\<Lambda> \<turnstile> \<rhd> \<cdot> v \<leadsto> \<epsilon> \<cdot> InlV (PairV v\<^sub>1 v\<^sub>2)" by simp
+        thus ?thesis by fastforce
+      next case False
+        with V have "\<Lambda> \<turnstile> \<rhd> \<cdot> v \<leadsto> \<epsilon> \<cdot> InrV (PairV v\<^sub>1 v\<^sub>2)" by simp
+        thus ?thesis by fastforce
+      qed
+  next case tc_app
+    then obtain e v' where V: "v = PairV (FunV e) v'" using canonical_prod canonical_arrow by blast
+    moreover hence "\<Lambda> \<turnstile> $ \<cdot> v \<leadsto> e \<cdot> v'" by simp
+    ultimately show ?case by fastforce
+  next case (tc_arr \<Gamma> f t\<^sub>1 t\<^sub>2 g)
+    then obtain e where "v = FunV e" using canonical_arrow by blast
+    moreover hence "\<Lambda> \<turnstile> g \<leftarrow> f \<cdot> FunV e \<leadsto> \<epsilon> \<cdot> FunV (g \<cdot> e \<cdot> f)" by simp
+    ultimately show ?case by fastforce
+  next case (tc_inj \<Gamma> n)
+    hence "\<Lambda> \<turnstile> \<succ>\<^bsub>n\<^esub> \<cdot> v \<leadsto> \<epsilon> \<cdot> InjV n v" by simp
+    thus ?case by fastforce
+  next case (tc_outj \<Gamma> n F)
+    then obtain v' m where "v = InjV m v' \<and> var\<^sub>t_type \<Gamma> m = Some F" using canonical_mu by blast
+    moreover hence "\<Lambda> \<turnstile> \<prec>\<^bsub>n\<^esub> \<cdot> v \<leadsto> \<epsilon> \<cdot> v'" by simp
+    ultimately show ?case by fastforce
+  next case (tc_cata \<Gamma> n F f t)
+    hence "var\<^sub>t_bind \<Lambda> n = Some F" by (simp add: typecheck_environment_def)
+    hence "\<Lambda> \<turnstile> \<lparr> f \<rparr>\<^bsub>n\<^esub> \<cdot> v \<leadsto> (f \<cdot> \<lparr> f \<rparr>\<^bsub>n\<^esub> \<bullet> F \<cdot> \<prec>\<^bsub>n\<^esub>) \<cdot> v" by simp
+    thus ?case by fastforce
+  next case (tc_ana \<Gamma> n F f t)
+    hence "var\<^sub>t_bind \<Lambda> n = Some F" by (simp add: typecheck_environment_def)
+    hence "\<Lambda> \<turnstile> \<lbrakk> f \<rbrakk>\<^bsub>n\<^esub> \<cdot> v \<leadsto> (\<succ>\<^bsub>n\<^esub> \<cdot> \<lbrakk> f \<rbrakk>\<^bsub>n\<^esub> \<bullet> F \<cdot> f) \<cdot> v" by simp
+    thus ?case by fastforce
+  next case (tc_var \<Gamma> x t\<^sub>1 t\<^sub>2)
+    then obtain e where "var\<^sub>e_bind \<Lambda> x = Some e \<and> \<Gamma> \<turnstile> e : t\<^sub>1 \<rightarrow> t\<^sub>2" 
+      using typecheck_environment_def typecheck_env\<^sub>e_def by fastforce
+    hence "\<Lambda> \<turnstile> Var x \<cdot> v \<leadsto> e \<cdot> v" by simp
+    thus ?case by fastforce
+  qed simp_all
 
 theorem progress [simp]: "\<Pi> \<TTurnstile> \<Gamma> \<rightarrow> t \<Longrightarrow> is_completed \<Pi> \<or> (\<exists>\<Pi>'. \<Pi> \<leadsto> \<Pi>')"
   proof (induction \<Pi> \<Gamma> t rule: typecheck_prog.induct)
@@ -579,6 +323,115 @@ theorem progress [simp]: "\<Pi> \<TTurnstile> \<Gamma> \<rightarrow> t \<Longrig
       qed simp_all
   qed
 
+(* preservation *)
+
+lemma [simp]: "\<Gamma> \<turnstile> e : t\<^sub>1 \<rightarrow> t\<^sub>2 \<Longrightarrow> \<Gamma> \<turnstile> e \<bullet> F : t\<^sub>1 \<star> F \<rightarrow> t\<^sub>2 \<star> F"
+  by (induction e F rule: apply_functor_expr.induct) simp_all
+
+theorem expr_preservation [simp]: "\<Lambda> \<turnstile> e \<cdot> v \<leadsto> e' \<cdot> v' \<Longrightarrow> \<Gamma> \<turnstile> e : t\<^sub>1 \<rightarrow> t\<^sub>2 \<Longrightarrow> 
+    \<Gamma> \<turnstile> v : t\<^sub>1 \<Longrightarrow> \<Gamma> \<tturnstile> \<Lambda> \<Longrightarrow> \<exists>t\<^sub>3. (\<Gamma> \<turnstile> e' : t\<^sub>3 \<rightarrow> t\<^sub>2) \<and> (\<Gamma> \<turnstile> v' : t\<^sub>3)"
+  proof (induction \<Lambda> e v e' v' arbitrary: t\<^sub>1 t\<^sub>2 rule: evaluate.induct)
+  case (ev_con \<Lambda> v\<^sub>1 v\<^sub>2)
+    hence "(\<Gamma> \<turnstile> \<epsilon> : t\<^sub>2 \<rightarrow> t\<^sub>2) \<and> \<Gamma> \<turnstile> v\<^sub>1 : t\<^sub>2" by fastforce
+    thus ?case by fastforce
+  next case (ev_comp1 \<Lambda> g v g' v' f)
+    moreover then obtain t\<^sub>3 where "(\<Gamma> \<turnstile> f : t\<^sub>3 \<rightarrow> t\<^sub>2) \<and> \<Gamma> \<turnstile> g : t\<^sub>1 \<rightarrow> t\<^sub>3" by fastforce
+    ultimately obtain t\<^sub>4 where "(\<Gamma> \<turnstile> f \<cdot> g' : t\<^sub>4 \<rightarrow> t\<^sub>2) \<and> \<Gamma> \<turnstile> v' : t\<^sub>4" by fastforce
+    thus ?case by fastforce
+  next case (ev_fst \<Lambda> v\<^sub>1 v\<^sub>2)
+    hence "(\<Gamma> \<turnstile> \<epsilon> : t\<^sub>2 \<rightarrow> t\<^sub>2) \<and> \<Gamma> \<turnstile> v\<^sub>1 : t\<^sub>2" by fastforce
+    thus ?case by fastforce
+  next case (ev_snd \<Lambda> v\<^sub>1 v\<^sub>2)
+    hence "(\<Gamma> \<turnstile> \<epsilon> : t\<^sub>2 \<rightarrow> t\<^sub>2) \<and> \<Gamma> \<turnstile> v\<^sub>2 : t\<^sub>2" by fastforce
+    thus ?case by fastforce
+  next case (ev_pair1 \<Lambda> f\<^sub>1 v\<^sub>1 f\<^sub>1' v\<^sub>1' f\<^sub>2 v\<^sub>2)
+    then obtain t\<^sub>1\<^sub>1 t\<^sub>1\<^sub>2 t\<^sub>2\<^sub>1 t\<^sub>2\<^sub>2 t\<^sub>1\<^sub>1' where T: "(\<Gamma> \<turnstile> v\<^sub>1 : t\<^sub>1\<^sub>1) \<and> (\<Gamma> \<turnstile> v\<^sub>2 : t\<^sub>1\<^sub>2) \<and> 
+      (\<Gamma> \<turnstile> f\<^sub>1 : t\<^sub>1\<^sub>1 \<rightarrow> t\<^sub>2\<^sub>1) \<and> (\<Gamma> \<turnstile> f\<^sub>2 : t\<^sub>1\<^sub>2 \<rightarrow> t\<^sub>2\<^sub>2) \<and> t\<^sub>1 = t\<^sub>1\<^sub>1 \<otimes> t\<^sub>1\<^sub>2 \<and> t\<^sub>2 = t\<^sub>2\<^sub>1 \<otimes> t\<^sub>2\<^sub>2 \<and> 
+        (\<Gamma> \<turnstile> f\<^sub>1' : t\<^sub>1\<^sub>1' \<rightarrow> t\<^sub>2\<^sub>1) \<and> \<Gamma> \<turnstile> v\<^sub>1' : t\<^sub>1\<^sub>1'" by fastforce
+    hence "(\<Gamma> \<turnstile> f\<^sub>1' \<parallel> f\<^sub>2 : t\<^sub>1\<^sub>1' \<otimes> t\<^sub>1\<^sub>2 \<rightarrow> t\<^sub>2) \<and> \<Gamma> \<turnstile> PairV v\<^sub>1' v\<^sub>2 : t\<^sub>1\<^sub>1' \<otimes> t\<^sub>1\<^sub>2" by simp
+    thus ?case by fastforce
+  next case (ev_pair2 \<Lambda> f\<^sub>2 v\<^sub>2 f\<^sub>2' v\<^sub>2' v\<^sub>1)
+    then obtain t\<^sub>1\<^sub>1 t\<^sub>1\<^sub>2 t\<^sub>2\<^sub>2 t\<^sub>1\<^sub>2' where T: "(\<Gamma> \<turnstile> v\<^sub>1 : t\<^sub>1\<^sub>1) \<and> (\<Gamma> \<turnstile> v\<^sub>2 : t\<^sub>1\<^sub>2) \<and> 
+      (\<Gamma> \<turnstile> f\<^sub>2 : t\<^sub>1\<^sub>2 \<rightarrow> t\<^sub>2\<^sub>2) \<and> t\<^sub>1 = t\<^sub>1\<^sub>1 \<otimes> t\<^sub>1\<^sub>2 \<and> t\<^sub>2 = t\<^sub>1\<^sub>1 \<otimes> t\<^sub>2\<^sub>2 \<and> (\<Gamma> \<turnstile> f\<^sub>2' : t\<^sub>1\<^sub>2' \<rightarrow> t\<^sub>2\<^sub>2) \<and> 
+        \<Gamma> \<turnstile> v\<^sub>2' : t\<^sub>1\<^sub>2'" by fastforce
+    hence "(\<Gamma> \<turnstile> \<epsilon> \<parallel> f\<^sub>2' : t\<^sub>1\<^sub>1 \<otimes> t\<^sub>1\<^sub>2' \<rightarrow> t\<^sub>2) \<and> \<Gamma> \<turnstile> PairV v\<^sub>1 v\<^sub>2' : t\<^sub>1\<^sub>1 \<otimes> t\<^sub>1\<^sub>2'" by simp
+    thus ?case by fastforce
+  next case (ev_pair3 \<Lambda> v\<^sub>1 v\<^sub>2)
+    hence "(\<Gamma> \<turnstile> \<epsilon> : t\<^sub>1 \<rightarrow> t\<^sub>2) \<and> \<Gamma> \<turnstile> PairV v\<^sub>1 v\<^sub>2 : t\<^sub>1" by fastforce
+    thus ?case by fastforce
+  next case (ev_tup \<Lambda> v)
+    hence "t\<^sub>2 = t\<^sub>1 \<otimes> t\<^sub>1" by fastforce
+    moreover from ev_tup have "(\<Gamma> \<turnstile> \<epsilon> : t\<^sub>1 \<otimes> t\<^sub>1 \<rightarrow> t\<^sub>1 \<otimes> t\<^sub>1) \<and> \<Gamma> \<turnstile> PairV v v : t\<^sub>1 \<otimes> t\<^sub>1" 
+      by simp
+    ultimately show ?case by fastforce
+  next case (ev_inl \<Lambda> v)
+    moreover then obtain t\<^sub>3 where "t\<^sub>2 = t\<^sub>1 \<oplus> t\<^sub>3" by fastforce
+    ultimately have "(\<Gamma> \<turnstile> \<epsilon> : t\<^sub>1 \<oplus> t\<^sub>3 \<rightarrow> t\<^sub>2) \<and> \<Gamma> \<turnstile> InlV v : t\<^sub>1 \<oplus> t\<^sub>3" by simp
+    thus ?case by fastforce
+  next case (ev_inr \<Lambda> v)
+    moreover then obtain t\<^sub>3 where "t\<^sub>2 = t\<^sub>3 \<oplus> t\<^sub>1" by fastforce
+    ultimately have "(\<Gamma> \<turnstile> \<epsilon> : t\<^sub>3 \<oplus> t\<^sub>1 \<rightarrow> t\<^sub>2) \<and> \<Gamma> \<turnstile> InrV v : t\<^sub>3 \<oplus> t\<^sub>1" by simp
+    thus ?case by fastforce
+  next case (ev_strl \<Lambda> v)
+    hence "(\<Gamma> \<turnstile> \<epsilon> : t\<^sub>2 \<rightarrow> t\<^sub>2) \<and> \<Gamma> \<turnstile> v : t\<^sub>2" by fastforce
+    thus ?case by fastforce
+  next case (ev_strr \<Lambda> v)
+    hence "(\<Gamma> \<turnstile> \<epsilon> : t\<^sub>2 \<rightarrow> t\<^sub>2) \<and> \<Gamma> \<turnstile> v : t\<^sub>2" by fastforce
+    thus ?case by fastforce
+  next case (ev_csl \<Lambda> f\<^sub>l f\<^sub>r v)
+    then obtain t\<^sub>1\<^sub>l t\<^sub>1\<^sub>r t\<^sub>2\<^sub>l t\<^sub>2\<^sub>r where V: "(\<Gamma> \<turnstile> f\<^sub>l : t\<^sub>1\<^sub>l \<rightarrow> t\<^sub>2\<^sub>l) \<and> (\<Gamma> \<turnstile> f\<^sub>r : t\<^sub>1\<^sub>r \<rightarrow> t\<^sub>2\<^sub>r) \<and> 
+      (\<Gamma> \<turnstile> v : t\<^sub>1\<^sub>l) \<and> t\<^sub>1 = t\<^sub>1\<^sub>l \<oplus> t\<^sub>1\<^sub>r \<and> t\<^sub>2 = t\<^sub>2\<^sub>l \<oplus> t\<^sub>2\<^sub>r" by fastforce
+    hence "\<Gamma> \<turnstile> \<iota>\<^sub>l \<cdot> f\<^sub>l : t\<^sub>1\<^sub>l \<rightarrow> t\<^sub>2\<^sub>l \<oplus> t\<^sub>2\<^sub>r" by (metis tc_inl tc_comp)
+    with V show ?case by fastforce
+  next case (ev_csr \<Lambda> f\<^sub>l f\<^sub>r v)
+    then obtain t\<^sub>1\<^sub>l t\<^sub>1\<^sub>r t\<^sub>2\<^sub>l t\<^sub>2\<^sub>r where V: "(\<Gamma> \<turnstile> f\<^sub>l : t\<^sub>1\<^sub>l \<rightarrow> t\<^sub>2\<^sub>l) \<and> (\<Gamma> \<turnstile> f\<^sub>r : t\<^sub>1\<^sub>r \<rightarrow> t\<^sub>2\<^sub>r) \<and> 
+      (\<Gamma> \<turnstile> v : t\<^sub>1\<^sub>r) \<and> t\<^sub>1 = t\<^sub>1\<^sub>l \<oplus> t\<^sub>1\<^sub>r \<and> t\<^sub>2 = t\<^sub>2\<^sub>l \<oplus> t\<^sub>2\<^sub>r" by fastforce
+    hence "\<Gamma> \<turnstile> \<iota>\<^sub>r \<cdot> f\<^sub>r : t\<^sub>1\<^sub>r \<rightarrow> t\<^sub>2\<^sub>l \<oplus> t\<^sub>2\<^sub>r" by (metis tc_inr tc_comp)
+    with V show ?case by fastforce
+  next case (ev_dstl \<Lambda> v\<^sub>1 v\<^sub>2)
+    then obtain t\<^sub>3 t\<^sub>4 t\<^sub>5 where "(\<Gamma> \<turnstile> v\<^sub>1 : t\<^sub>3) \<and> (\<Gamma> \<turnstile> v\<^sub>2 : t\<^sub>5) \<and> t\<^sub>1 = (t\<^sub>3 \<oplus> t\<^sub>4) \<otimes> t\<^sub>5 \<and> 
+      t\<^sub>2 = t\<^sub>3 \<otimes> t\<^sub>5 \<oplus> t\<^sub>4 \<otimes> t\<^sub>5" by fastforce
+    hence "(\<Gamma> \<turnstile> \<epsilon> : t\<^sub>2 \<rightarrow> t\<^sub>2) \<and> \<Gamma> \<turnstile> InlV (PairV v\<^sub>1 v\<^sub>2) : t\<^sub>2" by simp
+    thus ?case by fastforce
+  next case (ev_dstr \<Lambda> v\<^sub>1 v\<^sub>2)
+    then obtain t\<^sub>3 t\<^sub>4 t\<^sub>5 where "(\<Gamma> \<turnstile> v\<^sub>1 : t\<^sub>4) \<and> (\<Gamma> \<turnstile> v\<^sub>2 : t\<^sub>5) \<and> t\<^sub>1 = (t\<^sub>3 \<oplus> t\<^sub>4) \<otimes> t\<^sub>5 \<and> 
+      t\<^sub>2 = t\<^sub>3 \<otimes> t\<^sub>5 \<oplus> t\<^sub>4 \<otimes> t\<^sub>5" by fastforce
+    hence "(\<Gamma> \<turnstile> \<epsilon> : t\<^sub>2 \<rightarrow> t\<^sub>2) \<and> \<Gamma> \<turnstile> InrV (PairV v\<^sub>1 v\<^sub>2) : t\<^sub>2" by simp
+    thus ?case by fastforce
+  next case (ev_arr \<Lambda> g f e)
+    then obtain t\<^sub>1\<^sub>1 t\<^sub>1\<^sub>2 t\<^sub>2\<^sub>1 t\<^sub>2\<^sub>2 where "(\<Gamma> \<turnstile> f : t\<^sub>2\<^sub>1 \<rightarrow> t\<^sub>1\<^sub>1) \<and> (\<Gamma> \<turnstile> g : t\<^sub>1\<^sub>2 \<rightarrow> t\<^sub>2\<^sub>2) \<and> 
+      (\<Gamma> \<turnstile> e : t\<^sub>1\<^sub>1 \<rightarrow> t\<^sub>1\<^sub>2) \<and> t\<^sub>1 = t\<^sub>1\<^sub>1 \<hookrightarrow> t\<^sub>1\<^sub>2 \<and> t\<^sub>2 = t\<^sub>2\<^sub>1 \<hookrightarrow> t\<^sub>2\<^sub>2" by fastforce
+    hence "(\<Gamma> \<turnstile> \<epsilon> : t\<^sub>2\<^sub>1 \<hookrightarrow> t\<^sub>2\<^sub>2 \<rightarrow> t\<^sub>2) \<and> \<Gamma> \<turnstile> FunV (g \<cdot> e \<cdot> f) : t\<^sub>2\<^sub>1 \<hookrightarrow> t\<^sub>2\<^sub>2" by fastforce
+    thus ?case by fastforce
+  next case (ev_inj \<Lambda> F v)
+    hence "(\<Gamma> \<turnstile> \<epsilon> : t\<^sub>2 \<rightarrow> t\<^sub>2) \<and> \<Gamma> \<turnstile> InjV F v : t\<^sub>2" by fastforce
+    thus ?case by fastforce
+  next case (ev_outj \<Lambda> m F v)
+    hence "(\<Gamma> \<turnstile> \<epsilon> : t\<^sub>2 \<rightarrow> t\<^sub>2) \<and> \<Gamma> \<turnstile> v : t\<^sub>2" by fastforce
+    thus ?case by fastforce
+  next case (ev_cata \<Lambda> n F f v)
+    hence V: "(\<Gamma> \<turnstile> f : t\<^sub>2 \<star> F \<rightarrow> t\<^sub>2) \<and> \<Gamma> \<turnstile> v : \<mu> F" using typecheck_environment_def by fastforce
+    moreover from ev_cata have "\<Gamma> \<turnstile> \<lparr> f \<rparr>\<^bsub>n\<^esub> \<bullet> F : \<mu> F \<star> F \<rightarrow> t\<^sub>2 \<star> F" 
+      using typecheck_environment_def by fastforce
+    moreover from ev_cata have "\<Gamma> \<turnstile> \<prec>\<^bsub>n\<^esub> : \<mu> F \<rightarrow> \<mu> F \<star> F" using typecheck_environment_def by simp
+    ultimately have "\<Gamma> \<turnstile> f \<cdot> \<lparr> f \<rparr>\<^bsub>n\<^esub> \<bullet> F \<cdot> \<prec>\<^bsub>n\<^esub> : \<mu> F \<rightarrow> t\<^sub>2" by (metis tc_comp)
+    with V have "(\<Gamma> \<turnstile> f \<cdot> \<lparr> f \<rparr>\<^bsub>n\<^esub> \<bullet> F \<cdot> \<prec>\<^bsub>n\<^esub> : \<mu> F \<rightarrow> t\<^sub>2) \<and> \<Gamma> \<turnstile> v : \<mu> F" by simp
+    thus ?case by fastforce
+  next case (ev_ana \<Lambda> n F f v)
+    moreover hence V: "(\<Gamma> \<turnstile> f : t\<^sub>1 \<rightarrow> t\<^sub>1 \<star> F) \<and> (\<Gamma> \<turnstile> v : t\<^sub>1) \<and> t\<^sub>2 = \<mu> F"
+      using typecheck_environment_def by fastforce
+    ultimately have "\<Gamma> \<turnstile> \<succ>\<^bsub>n\<^esub> : t\<^sub>2 \<star> F \<rightarrow> t\<^sub>2" using typecheck_environment_def by simp
+    moreover from ev_ana have "\<Gamma> \<turnstile> \<lbrakk> f \<rbrakk>\<^bsub>n\<^esub> \<bullet> F : t\<^sub>1 \<star> F \<rightarrow> t\<^sub>2 \<star> F" by simp
+    moreover from V have "\<Gamma> \<turnstile> f : t\<^sub>1 \<rightarrow> t\<^sub>1 \<star> F" by simp
+    ultimately have "\<Gamma> \<turnstile> \<succ>\<^bsub>n\<^esub> \<cdot> \<lbrakk> f \<rbrakk>\<^bsub>n\<^esub> \<bullet> F \<cdot> f : t\<^sub>1 \<rightarrow> t\<^sub>2" by simp
+    with V show ?case by fastforce
+  next case (ev_var \<Lambda> x e v)
+    hence "var\<^sub>e_type \<Gamma> x = Some (t\<^sub>1, t\<^sub>2)" by fastforce
+    with ev_var obtain e' where "var\<^sub>e_bind \<Lambda> x = Some e' \<and> \<Gamma> \<turnstile> e' : t\<^sub>1 \<rightarrow> t\<^sub>2" 
+      using typecheck_environment_def typecheck_env\<^sub>e_def by fastforce 
+    with ev_var show ?case by fastforce
+  qed fastforce+
+
 theorem preservation [simp]: "\<Pi> \<leadsto> \<Pi>' \<Longrightarrow> \<Pi> \<TTurnstile> \<Gamma> \<rightarrow> t \<Longrightarrow> \<Pi>' \<TTurnstile> \<Gamma> \<rightarrow> t"
   proof (induction \<Pi> \<Pi>' rule: evaluate_prog.induct)
   case (ev_prog \<Lambda> e v e' v')
@@ -587,41 +440,5 @@ theorem preservation [simp]: "\<Pi> \<leadsto> \<Pi>' \<Longrightarrow> \<Pi> \<
     ultimately obtain t\<^sub>2 where "(\<Gamma> \<turnstile> e' : t\<^sub>2 \<rightarrow> t) \<and> (\<Gamma> \<turnstile> v' : t\<^sub>2)" by fastforce
     with T show ?case by fastforce
   qed
-
-(* big step evaluation *)
-
-inductive total_evaluate_prog :: "prog \<Rightarrow> val \<Rightarrow> bool" (infix "\<Down>" 60) where
-  ptev_base [simp]: "Prog \<Lambda> \<epsilon> v \<Down> v"
-| ptev_step [simp]: "Prog \<Lambda> e v \<leadsto> Prog \<Lambda> e' v' \<Longrightarrow> Prog \<Lambda> e' v' \<Down> v'' \<Longrightarrow> Prog \<Lambda> e v \<Down> v''"
-
-inductive total_evaluate_prog' :: "prog \<Rightarrow> val \<Rightarrow> bool" (infix "\<Down>\<Down>" 60) where
-  ptev_step' [simp]: "assemble_context \<Lambda> \<turnstile> e \<cdot> v \<Down> v' \<Longrightarrow> Prog \<Lambda> e v \<Down>\<Down> v'"
-
-inductive_cases [elim]: "Prog \<Lambda> e v \<Down>\<Down> v'"
-
-lemma [simp]: "\<Pi> \<Down> v = \<Pi> \<Down>\<Down> v"
-  proof
-    show "\<Pi> \<Down> v \<Longrightarrow> \<Pi> \<Down>\<Down> v" by (induction \<Pi> v rule: total_evaluate_prog.induct) fastforce+
-  next 
-    assume "\<Pi> \<Down>\<Down> v"
-    thus "\<Pi> \<Down> v"
-      proof (induction \<Pi> v rule: total_evaluate_prog'.induct)
-      case (ptev_step' \<Lambda> e v v')
-        thus ?case 
-          proof (induction "assemble_context \<Lambda>" e v v' rule: total_eval.induct)
-          case (tev_step e v e' v' v'')
-            moreover hence "Prog \<Lambda> e v \<leadsto> Prog \<Lambda> e' v'" by simp
-            ultimately show ?case by (metis total_evaluate_prog.ptev_step)
-          qed simp_all
-      qed
-  qed
-
-(* since we are a turing-complete language, total progress is not provable *)
-
-lemma [simp]: "\<Pi> \<Down>\<Down> v \<Longrightarrow> \<Pi> \<TTurnstile> \<Gamma> \<rightarrow> t \<Longrightarrow> \<Gamma> \<turnstile> v : t"
-  by (induction \<Pi> v rule: total_evaluate_prog'.induct) auto
-
-theorem total_preservation: "\<Pi> \<Down> v \<Longrightarrow> \<Pi> \<TTurnstile> \<Gamma> \<rightarrow> t \<Longrightarrow> \<Gamma> \<turnstile> v : t"
-  by simp
 
 end
